Iris/Iris/HeapLang/Lib/Increment.lean
@@ -1,0 +1,304 @@
+/-
+Copyright (c) 2026. All rights reserved.
+Released under Apache 2.0 license as described in the file LICENSE.
+Authors:
+-/
+module
+
+public import Iris.HeapLang.Lib.AtomicHeap
+public import Iris.HeapLang.Lib.Par
+public import Iris.Instances.Lib.Invariants
+
+@[expose] public section
+
+namespace Iris.HeapLang
+
+open BI Spawn Std Std.LawfulSet
+
+/-! # Fetch-and-add on top of compare-and-swap preserves logical atomicity -/
+
+/-! ## Logically atomic increment directly on top of the physical heap -/
+
+@[rocq_alias heap_lang.incr_phy]
+def incrPhy : Val := hl_val%
+  rec incr l :=
+    let oldv := !l;
+    if cas(l, oldv, oldv + #1) then oldv else incr l
+
+section IncrementPhysical
+
+variable [HeapLangGS hlc GF]
+
+@[rocq_alias heap_lang.incr_phy_spec]
+theorem incrPhy_spec (l : Loc) :
+    ⊢ iprop(<<{ ∀∀ (v : Int), l ↦ some hl_val(#v) }>> hl(&incrPhy #l) @ ∅
+      <<{ l ↦ some hl_val(#(v + 1 : Int)) | RET hl_val(#v) }>>) := by
+  iunfold atomic_wp
+  iintro %Φ AU
+  iloeb as IH
+  wp_rec
+  wp_bind !_
+  imod AU with ⟨%⟨v, ⟨⟩⟩, Hl, ⟨Hclose, -⟩⟩
+  isimp only [Tele.app] at Hl Hclose
+  wp_load
+  imod Hclose $$ Hl with AU
+  imodintro
+  wp_pures
+  wp_bind cmpXchg(_, _, _)
+  imod AU with ⟨%⟨w, ⟨⟩⟩, Hl, Hclose⟩
+  isimp only [Tele.app] at Hl Hclose
+  by_cases hw : v = w
+  · subst hw
+    wp_cmpxchg_suc
+    icases Hclose with ⟨-, Hclose⟩
+    imod Hclose $$ %Tele.Arg.nil [$Hl]
+    isimp only [Tele.bind, Tele.app, tforall_nil, BIBase.wandM] at Hclose
+    imodintro
+    wp_pures
+    iexact Hclose
+  · wp_cmpxchg_fail
+    · grind
+    icases Hclose with ⟨Hclose, -⟩
+    imod Hclose $$ Hl with AU
+    imodintro
+    wp_pures
+    isimp only [Tele.app] at IH
+    iapply IH $$ AU
+
+end IncrementPhysical
+
+/-! ## Logically atomic increment on top of an arbitrary logically atomic heap -/
+
+section Increment
+
+variable [IrisGS_gen hlc Exp GF] [A : AtomicHeap GF]
+
+@[rocq_alias heap_lang.increment.incr]
+def incr : Val := hl_val%
+  rec incr l :=
+    let oldv := &(A.load) l;
+    if snd(&(A.cmpXchg) l oldv (oldv + #1)) then oldv else incr l
+
+/-- A "weak increment": assumes that there is no race. -/
+@[rocq_alias heap_lang.weak_incr]
+def weakIncr : Val := hl_val%
+  rec weakIncr l :=
+    let oldv := &(A.load) l;
+    ((&(A.store) l (oldv + #1)); oldv)
+
+variable (H : A.atomicHeapG GF)
+
+/-- A proof of the `incr` specification that unfolds the definition of atomic accessors. This is
+the style that most logically atomic proofs take. -/
+@[rocq_alias heap_lang.incr_spec_direct]
+theorem incr_spec_direct (l : Loc) :
+    A.heapInv H ⊢ iprop(<<{ ∀∀ (v : Int), A.pointsTo H l (.own 1) hl_val(#v) }>>
+      hl(&(incr (A := A)) #l) @ (↑atomicHeapN)
+      <<{ A.pointsTo H l (.own 1) hl_val(#(v + 1 : Int)) | RET hl_val(#v) }>>) := by
+  iunfold atomic_wp
+  iintro #Hheap %Φ AU
+  iloeb as IH
+  wp_rec
+  awp_apply A.load_spec H l $$ Hheap
+  iunfold atomic_acc
+  imod AU with ⟨%⟨v, ⟨⟩⟩, Hl, ⟨Hclose, -⟩⟩
+  isimp only [Tele.app] at Hl Hclose
+  imodintro
+  iexists ⟨hl_val(#v), DFrac.own 1, .nil⟩
+  isimp only [Tele.app]
+  iframe Hl
+  isplit
+  · iexact Hclose
+  isimp only [Tele.bind, Tele.app, tforall_nil, BIBase.wandM]
+  iintro Hl
+  imod Hclose $$ Hl with AU
+  imodintro
+  wp_pures
+  awp_apply cas_spec H l hl_val(#v) hl_val(#(v + 1 : Int)) rfl $$ Hheap
+  iunfold atomic_acc
+  imod AU with ⟨%⟨w, ⟨⟩⟩, Hl, Hclose⟩
+  isimp only [Tele.app] at Hl Hclose
+  imodintro
+  iexists ⟨hl_val(#w), .nil⟩
+  isimp only [Tele.app]
+  iframe Hl
+  isplit
+  · icases Hclose with ⟨Hclose, -⟩
+    iexact Hclose
+  isimp only [Tele.bind, Tele.app, tforall_nil, BIBase.wandM]
+  iintro Hl
+  by_cases hw : w = v
+  · subst hw
+    icases Hclose with ⟨-, Hclose⟩
+    isimp only [↓reduceIte] at Hl
+    imod Hclose $$ %Tele.Arg.nil [$Hl]
+    imodintro
+    isimp only [Tele.bind, Tele.app, tforall_nil, BIBase.wandM] at Hclose
+    isimp only [↓reduceIte, decide_true]
+    wp_pures
+    iexact Hclose
+  · have hwv : (hl_val(#w) : Val) ≠ hl_val(#v) := by simp [hw]
+    icases Hclose with ⟨Hclose, -⟩
+    isimp only [hwv, ↓reduceIte] at Hl
+    imod Hclose $$ Hl with AU
+    imodintro
+    isimp only [hwv, ↓reduceIte, decide_false]
+    wp_pures
+    isimp only [Tele.app] at IH
+    iapply IH $$ AU
+
+/-- A proof of the `incr` specification that uses the `aacc_aupd_*` lemmas to avoid reasoning
+with the definition of atomic accessors. These lemmas are only usable here because the atomic
+update we have and the one we try to prove are in 1:1 correspondence; most logically atomic
+proofs will not be able to use them. -/
+@[rocq_alias heap_lang.incr_spec]
+theorem incr_spec (l : Loc) :
+    A.heapInv H ⊢ iprop(<<{ ∀∀ (v : Int), A.pointsTo H l (.own 1) hl_val(#v) }>>
+      hl(&(incr (A := A)) #l) @ (↑atomicHeapN)
+      <<{ A.pointsTo H l (.own 1) hl_val(#(v + 1 : Int)) | RET hl_val(#v) }>>) := by
+  iunfold atomic_wp
+  iintro #Hheap %Φ AU
+  iloeb as IH
+  wp_rec
+  awp_apply A.load_spec H l $$ Hheap
+  iapply aacc_aupd_abort subset_refl $$ AU
+  iintro %⟨x, ⟨⟩⟩ Hα
+  isimp only [Tele.app] at Hα
+  iaaccintro %⟨hl_val(#x), DFrac.own 1, .nil⟩ [Hα]
+  · isimp only [Tele.app]
+    iexact Hα
+  · isimp only [Tele.app]
+    iintro $ !> AU !> //
+  · isimp only [Tele.app_bind, Tele.app, tforall_nil, BIBase.wandM]
+    iintro $ !> AU !>
+    wp_pures
+    awp_apply cas_spec H l hl_val(#x) hl_val(#(x + 1 : Int)) rfl $$ Hheap
+    iapply aacc_aupd subset_refl $$ AU
+    iintro %⟨x', ⟨⟩⟩ Hα
+    isimp only [Tele.app] at Hα
+    iaaccintro %⟨hl_val(#x'), .nil⟩ [Hα]
+    · isimp only [Tele.app]
+      iexact Hα
+    · isimp only [Tele.app]
+      iintro $ !> AU !> //
+    · isimp only [Tele.app_bind, Tele.app, texist_nil, tforall_nil, BIBase.wandM]
+      iintro Hβ !>
+      by_cases hx : x' = x
+      · subst hx
+        isimp only [↓reduceIte] at Hβ
+        isimp only [↓reduceIte, decide_true]
+        iright
+        iframe Hβ
+        iintro Hpost !>
+        wp_pures
+        iexact Hpost
+      · have hxv : (hl_val(#x') : Val) ≠ hl_val(#x) := by simp [hx]
+        isimp only [hxv, ↓reduceIte] at Hβ
+        isimp only [hxv, ↓reduceIte, decide_false]
+        ileft
+        iframe Hβ
+        iintro AU !>
+        wp_pures
+        isimp only [Tele.app, tforall_nil, BIBase.wandM] at IH
+        iapply IH $$ AU
+
+/-- Logically atomic spec for the weak increment. Also an example for what TaDA calls a "private
+precondition". -/
+@[rocq_alias heap_lang.weak_incr_spec]
+theorem weakIncr_spec (l : Loc) (v : Int) :
+    A.heapInv H ⊢ A.pointsTo H l (.own (Qp.half 1)) hl_val(#v) -∗
+      iprop(<<{ ∀∀ (v' : Int), A.pointsTo H l (.own (Qp.half 1)) hl_val(#v') }>>
+        hl(&(weakIncr (A := A)) #l) @ (↑atomicHeapN)
+        <<{ ⌜v = v'⌝ ∗ A.pointsTo H l (.own 1) hl_val(#(v + 1 : Int)) | RET hl_val(#v) }>>) := by
+  iunfold atomic_wp
+  iintro #Hheap Hl %Φ AU
+  wp_rec
+  ihave Hload := A.load_spec H l $$ Hheap
+  wp_apply atomic_wp_seq $$ Hload %_ %⟨hl_val(#v), DFrac.own (Qp.half 1), .nil⟩ [Hl]
+  · isimp only [Tele.app]
+    iexact Hl
+  isimp only [Tele.app, tforall_nil, BIBase.wandM]
+  iintro Hl
+  wp_pures
+  awp_apply A.store_spec H l hl_val(#(v + 1 : Int)) $$ Hheap
+  iapply aacc_aupd_commit subset_refl $$ AU
+  iintro %⟨x, ⟨⟩⟩ Hα
+  isimp only [Tele.app] at Hα
+  ihave %hvx := pointsTo_agree H l _ _ _ _ $$ Hl Hα
+  obtain rfl : x = v := by grind
+  icombine Hl Hα as Hl
+  iaaccintro %⟨hl_val(#x), .nil⟩ [Hl]
+  · isimp only [Tele.app]
+    iexact Hl
+  · isimp only [Tele.app]
+    iintro ⟨$, Hl2⟩ !> AU !>
+    iframe AU Hl2
+  · isimp only [Tele.app_bind, Tele.app, texist_nil, tforall_nil, BIBase.wandM]
+    iintro Hβ !>
+    iframe Hβ
+    iintro HΦ !>
+    wp_pures
+    iexact HΦ
+
+end Increment
+
+/-! ## A client of the logically atomic increment -/
+
+section IncrementClient
+
+variable [HeapLangGS hlc GF] [SpawnG GF]
+
+/- The client runs against the physical heap, so that is the `AtomicHeap` instance `incr`
+resolves to for the rest of this section. -/
+attribute [local instance] primitiveAtomicHeap
+
+@[rocq_alias heap_lang.incr_client]
+def incrClient : Val := hl_val%
+  λ x,
+    let l := &((primitiveAtomicHeap (GF := GF)).alloc) x;
+    (&(incr (GF := GF)) l ‖ &(incr (GF := GF)) l)
+
+@[rocq_alias heap_lang.incr_client_safe]
+theorem incrClient_safe (x : Int) :
+    (primitiveAtomicHeap (GF := GF)).heapInv () ⊢
+      WP hl(&(incrClient (GF := GF)) #x) {{ _v, (True : IProp GF) }} := by
+  iintro #Hheap
+  wp_rec
+  wp_apply (primitiveAtomicHeap (GF := GF)).alloc_spec () hl_val(#x) $$ Hheap [//] with %l Hl
+  wp_pures
+  imod inv_alloc (nroot .@ "incr_client") ⊤
+    iprop(∃ x' : Int, (primitiveAtomicHeap (GF := GF)).pointsTo () l (.own 1) hl_val(#x'))
+    $$ [$Hl] with #Hinv
+  ihave #Aupd : iprop(□ WP hl(&(incr (GF := GF)) #l) {{ _v, (True : IProp GF) }}) $$ []
+  · iintro !>
+    awp_apply incr_spec (A := primitiveAtomicHeap (GF := GF)) () l $$ Hheap
+    iinv Hinv with ⟨%x', >Hl⟩
+    · refine ⟨fun p hp => mem_diff.mpr ⟨CoPset.mem_full, fun h => ?_⟩, trivial⟩
+      exact ndot_ne_disjoint nroot (x := "incr_client") (y := "atomic_heap") (by decide) p ⟨hp, h⟩
+    iaaccintro %⟨x', .nil⟩ [Hl]
+    · isimp only [Tele.app]
+      iexact Hl
+    · isimp only [Tele.app]
+      iintro Hl !>
+      isplitl [Hl]
+      · inext
+        iexists x'
+        iframe Hl
+      iempintro
+    · isimp only [Tele.app_bind, Tele.app, tforall_nil, BIBase.wandM]
+      iintro Hl !>
+      isplitl [Hl]
+      · inext
+        iexists x' + 1
+        iframe Hl
+      itrivial
+  iapply Par.wp_par (fun _ => iprop(True)) (fun _ => iprop(True)) $$ Aupd Aupd
+  · iintro %v₁ %v₂ _
+    inext
+    itrivial
+
+end IncrementClient
+
+end Iris.HeapLang
+
+end
